Added type names to expressions, started into programs

BananasProgram.thy
@@ -3,45 +3,59 @@ imports BananasExpression
 begin
 
 datatype decl = 
-  TypeDecl name funct
+  TypeDecl name "(name \<times> type list) list"
 | ExprDecl name expr
 
-primrec "binder" :: "decl \<Rightarrow> name set" where
-  "binder (TypeDecl x F) = {}"
-| "binder (ExprDecl x e) = {x}"
+primrec binders\<^sub>d :: "decl \<Rightarrow> name set" where
+  "binders\<^sub>d (TypeDecl x cts) = fst ` set cts"
+| "binders\<^sub>d (ExprDecl x e) = {x}"
 
 fun binders :: "decl list \<Rightarrow> name set" where
-  "binders \<Lambda> = \<Union> (binder ` set \<Lambda>)"
+  "binders \<Lambda> = \<Union> (binders\<^sub>d ` set \<Lambda>)"
 
-datatype prog = 
-  Prog "decl list" expr val
+datatype prog = Prog "decl list" expr val
 
-inductive typecheck_decl :: "(name \<rightharpoonup> type \<times> type) \<Rightarrow> decl \<Rightarrow> (name \<rightharpoonup> type \<times> type) \<Rightarrow> bool" 
-    (infix "\<Turnstile> _ :" 60) where
-  tcd_type [simp]: "\<Gamma> \<Turnstile> TypeDecl x F : \<Gamma>"
-| tcd_expr [simp]: "\<Gamma> \<turnstile> e : t\<^sub>1 \<rightarrow> t\<^sub>2 \<Longrightarrow> \<Gamma> \<Turnstile> ExprDecl x e : \<Gamma>(x \<mapsto> (t\<^sub>1, t\<^sub>2))"
+fun typecheck\<^sub>c :: "(name \<times> type list) list \<Rightarrow> (name \<rightharpoonup> type) \<times> funct" where
+  "typecheck\<^sub>c [] = (Map.empty, K \<zero>)" 
+| "typecheck\<^sub>c ((x, ts) # cts) = (
+    let (\<Gamma>, Fs) = typecheck\<^sub>c cts
+    in (\<Gamma>(x \<mapsto> foldr (op \<otimes>) ts \<one>), Fs \<Oplus> (foldr (\<lambda>t f. K t \<Otimes> f) ts (K \<one>))))"
 
-inductive_cases [elim]: "\<Gamma> \<Turnstile> TypeDecl x F : \<Gamma>'"
-inductive_cases [elim]: "\<Gamma> \<Turnstile> ExprDecl x e : \<Gamma>'"
+fun bind_with_names :: "name \<Rightarrow> (name \<rightharpoonup> type) \<Rightarrow> name \<rightharpoonup> type \<times> type" where
+  "bind_with_names n \<Gamma> x = map_option (\<lambda>t. (t, Named n)) (\<Gamma> x)"
 
-inductive typecheck_decls :: "(name \<rightharpoonup> type \<times> type) \<Rightarrow> decl list \<Rightarrow> (name \<rightharpoonup> type \<times> type) \<Rightarrow> bool" 
-    (infix "\<Turnstile> _ ::" 60) where
-  tcd_nil [simp]: "\<Gamma> \<Turnstile> [] :: \<Gamma>"
-| tcd_cons [simp]: "\<Gamma> \<Turnstile> \<delta> : \<Gamma>' \<Longrightarrow> binder \<delta> \<inter> binders \<Lambda> = {} \<Longrightarrow> \<Gamma>' \<Turnstile> \<Lambda> :: \<Gamma>'' \<Longrightarrow> 
-    \<Gamma> \<Turnstile> \<delta> # \<Lambda> :: \<Gamma>''"
+inductive typecheck_decl :: "(name \<rightharpoonup> type \<times> type) \<Rightarrow> (name \<rightharpoonup> funct) \<Rightarrow> decl \<Rightarrow> 
+    (name \<rightharpoonup> type \<times> type) \<Rightarrow> (name \<rightharpoonup> funct) \<Rightarrow> bool" (infix " & _ \<Turnstile> _ : _ &" 60) where
+  tcd_type [simp]: "typecheck\<^sub>c cts = (\<Gamma>', F) \<Longrightarrow> 
+    \<Gamma> & \<Sigma> \<Turnstile> TypeDecl x cts : \<Gamma> ++ bind_with_names x \<Gamma>' & \<Sigma>(x \<mapsto> F)"
+| tcd_expr [simp]: "\<Gamma> & \<Sigma> \<turnstile> e : t\<^sub>1 \<rightarrow> t\<^sub>2 \<Longrightarrow> \<Gamma> & \<Sigma> \<Turnstile> ExprDecl x e : \<Gamma>(x \<mapsto> (t\<^sub>1, t\<^sub>2)) & \<Sigma>"
 
-inductive_cases [elim]: "\<Gamma> \<Turnstile> [] :: \<Gamma>'"
-inductive_cases [elim]: "\<Gamma> \<Turnstile> \<delta> # \<Lambda> :: \<Gamma>'"
+inductive_cases [elim]: "\<Gamma> & \<Sigma> \<Turnstile> TypeDecl x F : \<Gamma>' & \<Sigma>'"
+inductive_cases [elim]: "\<Gamma> & \<Sigma> \<Turnstile> ExprDecl x e : \<Gamma>' & \<Sigma>'"
 
-inductive typecheck_prog :: "prog \<Rightarrow> (name \<rightharpoonup> type \<times> type) \<Rightarrow> type \<Rightarrow> bool" 
-    (infix "\<TTurnstile> _ :" 60) where
-  tcp_prog [simp]: "Map.empty \<Turnstile> \<Lambda> :: \<Gamma> \<Longrightarrow> \<Gamma> \<turnstile> e : t\<^sub>1 \<rightarrow> t\<^sub>2 \<Longrightarrow> \<Gamma> \<turnstile> v : t\<^sub>1 \<Longrightarrow> 
-    Prog \<Lambda> e v \<TTurnstile> \<Gamma> : t\<^sub>2"
+inductive typecheck_decls :: "(name \<rightharpoonup> type \<times> type) \<Rightarrow> (name \<rightharpoonup> funct) \<Rightarrow> decl list \<Rightarrow> 
+    (name \<rightharpoonup> type \<times> type) \<Rightarrow> (name \<rightharpoonup> funct) \<Rightarrow> bool" (infix "& _ \<Turnstile> _ :: _ &" 60) where
+  tcd_nil [simp]: "\<Gamma> & \<Sigma> \<Turnstile> [] :: \<Gamma> & \<Sigma>"
+| tcd_cons [simp]: "\<Gamma> & \<Sigma> \<Turnstile> \<delta> : \<Gamma>' & \<Sigma>' \<Longrightarrow> binders\<^sub>d \<delta> \<inter> binders \<Lambda> = {} \<Longrightarrow> 
+    \<Gamma>' & \<Sigma> \<Turnstile> \<Lambda> :: \<Gamma>'' & \<Sigma>'' \<Longrightarrow> \<Gamma> & \<Sigma> \<Turnstile> \<delta> # \<Lambda> :: \<Gamma>'' & \<Sigma>''"
 
-inductive_cases [elim]: "Prog \<Lambda> e v \<TTurnstile> \<Gamma> : t"
+inductive_cases [elim]: "\<Gamma> & \<Sigma> \<Turnstile> [] :: \<Gamma>' & \<Sigma>'"
+inductive_cases [elim]: "\<Gamma> & \<Sigma> \<Turnstile> \<delta> # \<Lambda> :: \<Gamma>' & \<Sigma>'"
+
+inductive typecheck_prog :: "prog \<Rightarrow> (name \<rightharpoonup> type \<times> type) \<Rightarrow> (name \<rightharpoonup> funct) \<Rightarrow> type \<Rightarrow> bool" 
+    (infix "\<TTurnstile> _ & _ :" 60) where
+  tcp_prog [simp]: "Map.empty & Map.empty \<Turnstile> \<Lambda> :: \<Gamma> & \<Sigma> \<Longrightarrow> \<Gamma> & \<Sigma> \<turnstile> e : t\<^sub>1 \<rightarrow> t\<^sub>2 \<Longrightarrow> 
+    \<Gamma> & \<Sigma> \<turnstile> v : t\<^sub>1 \<Longrightarrow> Prog \<Lambda> e v \<TTurnstile> \<Gamma> & \<Sigma> : t\<^sub>2"
+
+inductive_cases [elim]: "Prog \<Lambda> e v \<TTurnstile> \<Gamma> & \<Sigma> : t"
+
+fun assemble_context\<^sub>c :: "name \<Rightarrow> (name \<times> type list) list \<Rightarrow> name \<rightharpoonup> expr" where
+  "assemble_context\<^sub>c n [] = Map.empty"
+| "assemble_context\<^sub>c n ((x, t) # cts) = 
+    (map_option (op \<cdot> \<iota>\<^sub>r) o assemble_context\<^sub>c n cts)(x \<mapsto> \<prec>\<^bsub>n\<^esub> \<cdot> \<iota>\<^sub>l)"
 
 primrec assemble_context' :: "decl \<Rightarrow> name \<rightharpoonup> expr" where
-  "assemble_context' (TypeDecl x F) = Map.empty"
+  "assemble_context' (TypeDecl x cts) = assemble_context\<^sub>c x cts"
 | "assemble_context' (ExprDecl x e) = [x \<mapsto> e]"
 
 primrec assemble_context :: "decl list \<Rightarrow> name \<rightharpoonup> expr" where
@@ -52,7 +66,7 @@ primrec is_completed :: "prog \<Rightarrow> bool" where
   "is_completed (Prog \<Lambda> e v) = (e = \<epsilon>)"
 
 inductive evaluate_prog :: "prog \<Rightarrow> prog \<Rightarrow> bool" (infix "\<leadsto>" 60) where
-  ev_prog [simp]: "assemble_context \<Lambda> \<turnstile> e \<cdot> v \<leadsto> e' \<cdot> v' \<Longrightarrow> Prog \<Lambda> e v \<leadsto> Prog \<Lambda> e' v'"
+  ev_prog [simp]: "assemble_context \<Lambda> & \<Sigma> \<turnstile> e \<cdot> v \<leadsto> e' \<cdot> v' \<Longrightarrow> Prog \<Lambda> e v \<leadsto> Prog \<Lambda> e' v'"
 
 inductive_cases [elim]: "Prog \<Lambda> e v \<leadsto> \<Pi>"
 
@@ -61,58 +75,100 @@ inductive_cases [elim]: "Prog \<Lambda> e v \<leadsto> \<Pi>"
 lemma [simp]: "assemble_context (\<Lambda> @ \<Lambda>') = assemble_context \<Lambda> ++ assemble_context \<Lambda>'"
   by (induction \<Lambda>) simp_all
 
-lemma [simp]: "x \<notin> binder a \<Longrightarrow> x \<notin> dom (assemble_context' a)"
+lemma [simp]: "x \<notin> fst ` set cts \<Longrightarrow> x \<notin> dom (assemble_context\<^sub>c F cts)"
+  by (induction cts rule: assemble_context\<^sub>c.induct) simp_all
+
+lemma [simp]: "x \<notin> binders\<^sub>d a \<Longrightarrow> x \<notin> dom (assemble_context' a)"
   by (induction a) simp_all
 
 lemma [simp]: "x \<notin> binders \<Lambda> \<Longrightarrow> x \<notin> dom (assemble_context \<Lambda>)"
   by (induction \<Lambda>) simp_all
 
-lemma [simp]: "\<Gamma> \<turnstile> e : t\<^sub>1 \<rightarrow> t\<^sub>2 \<Longrightarrow> \<Gamma> \<tturnstile> \<Lambda> \<Longrightarrow> x \<notin> dom \<Lambda> \<Longrightarrow> \<Gamma>(x \<mapsto> (t\<^sub>1, t\<^sub>2)) \<tturnstile> \<Lambda>(x \<mapsto> e)"
+lemma [simp]: "\<Gamma> & \<Sigma> \<turnstile> e : t\<^sub>1 \<rightarrow> t\<^sub>2 \<Longrightarrow> \<Gamma> & \<Sigma> \<tturnstile> \<Lambda> \<Longrightarrow> x \<notin> dom \<Lambda> \<Longrightarrow> 
+    \<Gamma>(x \<mapsto> (t\<^sub>1, t\<^sub>2)) & \<Sigma> \<tturnstile> \<Lambda>(x \<mapsto> e)"
   proof (unfold typecheck_context_def, rule, rule, rule, rule)
     fix y t\<^sub>1' t\<^sub>2'
-    assume A: "\<Gamma> \<turnstile> e : t\<^sub>1 \<rightarrow> t\<^sub>2"
-       and B: "\<forall>x t\<^sub>1 t\<^sub>2. \<Gamma> x = Some (t\<^sub>1, t\<^sub>2) \<longrightarrow> (\<exists>e. \<Lambda> x = Some e \<and> \<Gamma> \<turnstile> e : t\<^sub>1 \<rightarrow> t\<^sub>2)"
+    assume A: "\<Gamma> & \<Sigma> \<turnstile> e : t\<^sub>1 \<rightarrow> t\<^sub>2"
+       and B: "\<forall>x t\<^sub>1 t\<^sub>2. \<Gamma> x = Some (t\<^sub>1, t\<^sub>2) \<longrightarrow> (\<exists>e. \<Lambda> x = Some e \<and> \<Gamma> & \<Sigma> \<turnstile> e : t\<^sub>1 \<rightarrow> t\<^sub>2)"
        and C: "x \<notin> dom \<Lambda>"
        and D: "(\<Gamma>(x \<mapsto> (t\<^sub>1, t\<^sub>2))) y = Some (t\<^sub>1', t\<^sub>2')"
     moreover hence E: "x \<notin> dom \<Gamma>" by auto
-    ultimately show "\<exists>e'. (\<Lambda>(x \<mapsto> e)) y = Some e' \<and> \<Gamma>(x \<mapsto> (t\<^sub>1, t\<^sub>2)) \<turnstile> e' : t\<^sub>1' \<rightarrow> t\<^sub>2'"
+    ultimately show "\<exists>e'. (\<Lambda>(x \<mapsto> e)) y = Some e' \<and> \<Gamma>(x \<mapsto> (t\<^sub>1, t\<^sub>2)) & \<Sigma> \<turnstile> e' : t\<^sub>1' \<rightarrow> t\<^sub>2'"
       proof (cases "x = y")
       case False
-        with B D obtain e' where "\<Lambda> y = Some e' \<and> \<Gamma> \<turnstile> e' : t\<^sub>1' \<rightarrow> t\<^sub>2'" by fastforce
+        with B D obtain e' where "\<Lambda> y = Some e' \<and> \<Gamma> & \<Sigma> \<turnstile> e' : t\<^sub>1' \<rightarrow> t\<^sub>2'" by fastforce
         with E False show ?thesis by simp
       qed simp_all
   qed
 
-lemma assemble_postpend: "\<Gamma> \<Turnstile> \<delta> : \<Gamma>' \<Longrightarrow> \<Gamma> \<tturnstile> assemble_context \<Lambda> \<Longrightarrow> binder \<delta> \<inter> binders \<Lambda> = {} \<Longrightarrow> 
-    \<Gamma>' \<tturnstile> assemble_context (\<Lambda> @ [\<delta>])"
-  proof (induction \<Gamma> \<delta> \<Gamma>' rule: typecheck_decl.induct)
-  case (tcd_expr \<Gamma> e t\<^sub>1 t\<^sub>2 x)
+lemma [simp]: "bind_with_names x Map.empty = Map.empty"
+  by auto
+
+lemma [simp]: "bind_with_names x (\<Gamma>(y \<mapsto> t)) = (bind_with_names x \<Gamma>)(y \<mapsto> (t, Named x))"
+  by auto
+
+lemma add_constructors: "typecheck\<^sub>c cts = (\<Gamma>', F) \<Longrightarrow> \<Gamma> & \<Sigma> \<tturnstile> assemble_context \<Lambda> \<Longrightarrow> 
+  fst ` set cts \<inter> binders \<Lambda> = {} \<Longrightarrow> 
+    \<Gamma> ++ bind_with_names x \<Gamma>' & \<Sigma> \<tturnstile> assemble_context \<Lambda> ++ assemble_context\<^sub>c F cts"
+  proof (induction cts arbitrary: \<Gamma>' F rule: typecheck\<^sub>c.induct)
+  case (2 y ts cts)
+    then obtain \<Gamma>'' Fs where G: "typecheck\<^sub>c cts = (\<Gamma>'', Fs) \<and> \<Gamma>' = \<Gamma>''(y \<mapsto> foldr op \<otimes> ts \<one>) \<and> 
+      F = Fs \<Oplus> foldr (\<lambda>t. op \<Otimes> (K t)) ts (K \<one>)" by (auto split: prod.splits)
+    with 2 have "\<Gamma> ++ bind_with_names x \<Gamma>'' \<tturnstile> assemble_context \<Lambda> ++ assemble_context\<^sub>c Fs cts" by fastforce
+
+    let ?t = "foldr op \<otimes> ts \<one>"
+    let ?F = "Fs \<Oplus> foldr (\<lambda>t. op \<Otimes> (K t)) ts (K \<one>)"
+    let ?\<Lambda> = "assemble_context \<Lambda>"
+
+
+    from 2 have "\<Gamma> \<tturnstile> assemble_context \<Lambda>" by simp
+    from 2 have "y \<notin> binders \<Lambda>" by simp
+    from 2 have "fst ` set cts \<inter> binders \<Lambda> = {}" by simp
+
+
+    have X: "(\<Gamma> ++ bind_with_names x \<Gamma>'') \<turnstile> \<prec>\<^bsub>?F\<^esub> \<cdot> \<iota>\<^sub>l : ?t \<rightarrow> Named x" by simp
+
+
+    have Y: "(\<Gamma> ++ bind_with_names x \<Gamma>'') \<tturnstile> (?\<Lambda> ++ (map_option (op \<cdot> \<iota>\<^sub>r) \<circ> assemble_context\<^sub>c ?F cts))" by simp
+
+
+    have "y \<notin> dom (?\<Lambda> ++ (map_option (op \<cdot> \<iota>\<^sub>r) \<circ> assemble_context\<^sub>c ?F cts))" by simp
+    with X Y G have "\<Gamma> ++ bind_with_names x \<Gamma>' \<tturnstile> ?\<Lambda> ++ assemble_context\<^sub>c F ((y, ts) # cts)" by simp
+    thus ?case by blast
+  qed auto
+
+lemma assemble_postpend: "\<Gamma> & \<Sigma> \<Turnstile> \<delta> : \<Gamma>' & \<Sigma>' \<Longrightarrow> \<Gamma> \<tturnstile> assemble_context \<Lambda> \<Longrightarrow> 
+    binders\<^sub>d \<delta> \<inter> binders \<Lambda> = {} \<Longrightarrow> \<Gamma>' \<tturnstile> assemble_context (\<Lambda> @ [\<delta>])"
+  proof (induction \<Gamma> \<Sigma> \<delta> \<Gamma>' \<Sigma>' rule: typecheck_decl.induct)
+  case tcd_type
+    thus ?case using add_constructors by simp
+  next case (tcd_expr \<Gamma> e t\<^sub>1 t\<^sub>2 \<Sigma> x)
     hence "\<Gamma>(x \<mapsto> (t\<^sub>1, t\<^sub>2)) \<tturnstile> assemble_context (\<Lambda> @ [ExprDecl x e])" by simp
     thus ?case by blast
-  qed simp_all
+  qed
 
-lemma tc_assemble_context [simp]: "\<Gamma> \<Turnstile> \<Lambda>' :: \<Gamma>' \<Longrightarrow> \<Gamma> \<tturnstile> assemble_context \<Lambda> \<Longrightarrow> 
+lemma tc_assemble_context [simp]: "\<Gamma> & \<Sigma> \<Turnstile> \<Lambda>' :: \<Gamma>' & \<Sigma>' \<Longrightarrow> \<Gamma> \<tturnstile> assemble_context \<Lambda> \<Longrightarrow> 
     binders \<Lambda> \<inter> binders \<Lambda>' = {} \<Longrightarrow> \<Gamma>' \<tturnstile> assemble_context \<Lambda> ++ assemble_context \<Lambda>'"
-  proof (induction \<Gamma> \<Lambda>' \<Gamma>' arbitrary: \<Lambda> rule: typecheck_decls.induct)
+  proof (induction \<Gamma> \<Sigma> \<Lambda>' \<Gamma>' \<Sigma>' arbitrary: \<Lambda> rule: typecheck_decls.induct)
   case tcd_nil
     thus ?case by simp
-  next case (tcd_cons \<Gamma> \<delta> \<Gamma>' \<Lambda>' \<Gamma>'')
+  next case (tcd_cons \<Gamma> \<Sigma> \<delta> \<Gamma>' \<Sigma>' \<Lambda>' \<Gamma>'')
     moreover hence "\<Gamma>' \<tturnstile> assemble_context (\<Lambda> @ [\<delta>])" using assemble_postpend by fastforce
     moreover from tcd_cons have "binders (\<Lambda> @ [\<delta>]) \<inter> binders \<Lambda>' = {}" by auto
     ultimately have "\<Gamma>'' \<tturnstile> assemble_context (\<Lambda> @ [\<delta>]) ++ assemble_context \<Lambda>'" by blast
     thus ?case by simp
   qed
 
-lemma [simp]: "Map.empty \<Turnstile> \<Lambda> :: \<Gamma> \<Longrightarrow> \<Gamma> \<tturnstile> assemble_context \<Lambda>"
+lemma [simp]: "Map.empty & Map.empty \<Turnstile> \<Lambda> :: \<Gamma> & \<Sigma> \<Longrightarrow> \<Gamma> \<tturnstile> assemble_context \<Lambda>"
   proof -
-    assume "Map.empty \<Turnstile> \<Lambda> :: \<Gamma>"
+    assume "Map.empty & Map.empty \<Turnstile> \<Lambda> :: \<Gamma> & \<Sigma>"
     moreover have "Map.empty \<tturnstile> assemble_context []" by (simp add: typecheck_context_def)
     ultimately show "\<Gamma> \<tturnstile> assemble_context \<Lambda>" using tc_assemble_context by fastforce
   qed
 
-theorem progress [simp]: "\<Pi> \<TTurnstile> \<Gamma> : t \<Longrightarrow> is_completed \<Pi> \<or> (\<exists>\<Pi>'. \<Pi> \<leadsto> \<Pi>')"
-  proof (induction \<Pi> \<Gamma> t rule: typecheck_prog.induct)
-  case (tcp_prog \<Lambda> \<Gamma> e t\<^sub>1 t\<^sub>2 v)
+theorem progress [simp]: "\<Pi> \<TTurnstile> \<Gamma> & \<Sigma> : t \<Longrightarrow> is_completed \<Pi> \<or> (\<exists>\<Pi>'. \<Pi> \<leadsto> \<Pi>')"
+  proof (induction \<Pi> \<Gamma> \<Sigma> t rule: typecheck_prog.induct)
+  case (tcp_prog \<Lambda> \<Gamma> \<Sigma> e t\<^sub>1 t\<^sub>2 v)
     thus ?case 
       proof (cases "e = \<epsilon>")
       case False
@@ -122,10 +178,11 @@ theorem progress [simp]: "\<Pi> \<TTurnstile> \<Gamma> : t \<Longrightarrow> is_
       qed simp_all
   qed
 
-theorem preservation [simp]: "\<Pi> \<leadsto> \<Pi>' \<Longrightarrow> \<Pi> \<TTurnstile> \<Gamma> : t \<Longrightarrow> \<Pi>' \<TTurnstile> \<Gamma> : t"
+theorem preservation [simp]: "\<Pi> \<leadsto> \<Pi>' \<Longrightarrow> \<Pi> \<TTurnstile> \<Gamma> & \<Sigma> : t \<Longrightarrow> \<Pi>' \<TTurnstile> \<Gamma> & \<Sigma> : t"
   proof (induction \<Pi> \<Pi>' rule: evaluate_prog.induct)
   case (ev_prog \<Lambda> e v e' v')
-    then obtain t\<^sub>1 where "(Map.empty \<Turnstile> \<Lambda> :: \<Gamma>) \<and> (\<Gamma> \<turnstile> e : t\<^sub>1 \<rightarrow> t) \<and> \<Gamma> \<turnstile> v : t\<^sub>1" by fastforce
+    then obtain t\<^sub>1 where "(Map.empty & Map.empty \<Turnstile> \<Lambda> :: \<Gamma> & \<Sigma>) \<and> (\<Gamma> \<turnstile> e : t\<^sub>1 \<rightarrow> t) \<and> \<Gamma> \<turnstile> v : t\<^sub>1" 
+      by fastforce
     moreover with ev_prog obtain t\<^sub>3 where "(\<Gamma> \<turnstile> e' : t\<^sub>3 \<rightarrow> t) \<and> \<Gamma> \<turnstile> v' : t\<^sub>3" by fastforce
     ultimately show ?case by fastforce
   qed
@@ -160,10 +217,10 @@ lemma [simp]: "\<Pi> \<Down> v = \<Pi> \<Down>\<Down> v"
 
 (* since we are a turing-complete language, total progress is not provable *)
 
-lemma [simp]: "\<Pi> \<Down>\<Down> v \<Longrightarrow> \<Pi> \<TTurnstile> \<Gamma> : t \<Longrightarrow> \<Gamma> \<turnstile> v : t"
+lemma [simp]: "\<Pi> \<Down>\<Down> v \<Longrightarrow> \<Pi> \<TTurnstile> \<Gamma> & \<Sigma> : t \<Longrightarrow> \<Gamma> \<turnstile> v : t"
   by (induction \<Pi> v rule: total_evaluate_prog'.induct) auto
 
-theorem total_preservation: "\<Pi> \<Down> v \<Longrightarrow> \<Pi> \<TTurnstile> \<Gamma> : t \<Longrightarrow> \<Gamma> \<turnstile> v : t"
+theorem total_preservation: "\<Pi> \<Down> v \<Longrightarrow> \<Pi> \<TTurnstile> \<Gamma> & \<Sigma> : t \<Longrightarrow> \<Gamma> \<turnstile> v : t"
   by simp
 
 end
